\begin{enumerate}[(a)]
    \item 
    From the question, we can find that \[^s\omega=\begin{bmatrix}
        0\\1\\0\\
    \end{bmatrix}, {}^sv = \begin{bmatrix}
        0\\0\\0 \end{bmatrix}\]
    we can get \[^sV=\begin{bmatrix}
        ^s\omega \\ ^sv\\
    \end{bmatrix} = \begin{bmatrix}
        0\\1\\0\\0\\0\\0\\
    \end{bmatrix}\]
    Similarly, we can get\[{}^bV_b=\begin{bmatrix}
        0 \\ 0 \\ 1 \\ 0 \\ 10 \\ 0\\
    \end{bmatrix}\]
    And beacuse 
    \[{}^bV_s={}^bX_s{}^sV\]其中\[{}^bX_s = \begin{bmatrix}
        R & 0 \\ [p]R & R
    \end{bmatrix}\]
    As can be known from the figure,\[{}^bR_s = \begin{bmatrix}
        \cos t & \sin t & 0 \\
        -\sin t & \cos t & 0 \\
        0 & 0 & 1\\
    \end{bmatrix}, p = \begin{bmatrix}
        -10 \\ 0 \\ 20 \\ 
    \end{bmatrix}\]
    So we can get \[{}^bV = {}^bV_b + {}^bV_s = \begin{bmatrix}
        {}^b\omega \\ {}^bv
    \end{bmatrix}
    \begin{bmatrix}
        \sin t \\ \cos t \\ 1 \\ -20\cos t \\ 20\sin t + 10 \\ -10\cos t \\
    \end{bmatrix}\]
    Therefore, \[{}^b\omega = \begin{bmatrix}
        \sin t \\ \cos t \\ 1 \\
    \end{bmatrix},
    {}^bv = \begin{bmatrix}
    -20\cos t \\ 20\sin t + 10 \\ -10\cos t \\
    \end{bmatrix}
    \]
    \item 
    \[\dot{p} = {}^sR_bv_b = \begin{bmatrix}
        -20 \cos t - 20 \cos t \sin t \\ 10 \cos t \\ 20 \sin t + 10 \sin^2t- 10 \cos^2t \\
    \end{bmatrix}\]
\end{enumerate}