\begin{enumerate}[(a)]
    \item 
    From the geometric relationship, we can know that: \[{}^sP=(L+d \sin \theta) \hat{\mathrm{x}}_{\mathrm{s}}+(L-d \cos \theta) \hat{\mathrm{y}}_{\mathrm{s}} \]
    \item 
    the velocity of point P is : \[\frac{d_{{}^sP}}{d_t} = \begin{bmatrix}
        d\dot{\theta}\cos\theta\\ d\dot{\theta}\sin\theta \\ 0
    \end{bmatrix}\]
    \item 
    \[t_{sb} = {}^sT_b = \begin{bmatrix}
        {}^sR_b & P \\
        0 & 1\\
    \end{bmatrix} =
    \begin{bmatrix}
        \cos\theta & -\sin\theta & 0 & L+d\sin\theta \\
        \sin\theta & cos\theta & 0 & L-d\sin\theta \\
        0 & 0 & 1 & 0 \\
        0 & 0 & 0 & 1\\
    \end{bmatrix}\]
    \item 
    Because: 
    \[^bV = \begin{bmatrix}
        ^b\omega\\^bv_{ob}
    \end{bmatrix} \]
    where, \[^bv_{ob} = \omega * \overrightarrow{rob}\]
    so, \[^bV = \begin{bmatrix}^b\omega\\^bv_{ob}\end{bmatrix} = \begin{bmatrix}
    0 \\ 0 \\ \dot{\theta} \\ d\dot{\theta} \\ 0 \\ 0
    \end{bmatrix}\]
    \item 
    Similarly to (d) \[^sV = \begin{bmatrix}
    ^s\omega\\^sv_{os}
    \end{bmatrix} \]
    where, \[^sv_{os} = \omega * \overrightarrow{ros}\]
    so, \[^sV = \begin{bmatrix}^s\omega\\^sv_{os}\end{bmatrix} = \begin{bmatrix}
    0 \\ 0 \\ \dot{\theta} \\ L\dot{\theta} \\ -L\dot{\theta} \\ 0
    \end{bmatrix}\]
    \item 
    It can be concluded that \[^sV= ^sX_b * ^bV \]
    where, 
    \[^sX_b = ^sT_b = \begin{bmatrix}
        R & 0 \\ [p]R & R
    \end{bmatrix} \]
    \item 
    Because \(^bV_p = ^sR_b^{-1} * ^sV_p\), and \(^sR_b\text{is}T_{sb}\), this is the relationship between them.
    \item 
    Beacuse \(^sV_{os} = ^sV_p + ^s\omega \times \overrightarrow{opos}\)
\end{enumerate}