\begin{enumerate}[(a)]
    \item 
    From the figure, we know \(p_a = P_{ab} + r_a\), so\[r_a = p_a - P_{ab}\]
    Among them, \(P_{ab}\)can be derived from \(^AT_B\) as \(\begin{bmatrix} -100\\300\\500 \end{bmatrix}\)\\
    So \[r_a = \begin{bmatrix}100\\500\\-500 \\ \end{bmatrix}\]
    And because
    \[r_b = ^BR_A*r_a\]
    \[^BR_A={(^AR_B)}^{-1}= \begin{bmatrix} 0 & 1 & 0  \\ -1 & 0 & 0  \\ 0 & 0 & 1 \\ \end{bmatrix}\]
    So \[r_b = \begin{bmatrix}
        500 \\ -100 \\ -500
    \end{bmatrix}\]
    \item 
    From the figure, we know \[^AT_C = \begin{bmatrix}
        1 & 0 & 0 & 0\\
        0 & \frac{\sqrt{3}}{2} & -\frac{1}{2} & 800\\
        0 & \frac{1}{2} & \frac{\sqrt{3}}{2} & 0\\
        0 & 0 & 0 & 1
    \end{bmatrix}\]
    So, \[T_{bc} = ^BT_C = ^BT_A * ^AT_C = (^BT_A)^{-1} * ^AT_C = \begin{bmatrix}
        0 & \frac{\sqrt{3}}{2} & -\frac{1}{2} & 500\\
        -1 & 0 & 0 & -100 \\
        0 & \frac12 & \frac{\sqrt{3}}{2} & -500 \\
        0 & 0 & 0 & 1\\
    \end{bmatrix}\]
\end{enumerate}
